Cslib/Languages/LambdaCalculus/Named/Untyped/Properties.lean
@@ -21,37 +21,253 @@ namespace LambdaCalculus.Named
 open Term
 
 /-- A variable in a term is either free or bound. -/
-lemma Term.vars_either_fv_or_bv [DecidableEq Var] (m : Term Var) :
+lemma Term.vars_either_fv_or_bv [DecidableEq Var] {m : Term Var} :
     m.vars = m.fv ∪ m.bv := by
-  induction m <;> grind [Term.fv, Term.bv, Term.vars]
+  induction m <;> grind [fv, bv, vars]
 
 /-- Renaming an unused variable has no effect. -/
-lemma Term.rename_unused [DecidableEq Var] (m : Term Var) (x y : Var) :
+@[simp]
+lemma Term.rename_unused [DecidableEq Var] {m : Term Var} {x y : Var} :
   x ∉ m.vars → m.rename x y = m := by
-  induction m <;> grind [Term.vars, Term.rename]
+  induction m <;> grind [vars, rename]
 
-/-- Renaming changes the set of variables. -/
-lemma Term.rename_vars [DecidableEq Var] (m : Term Var) (x y : Var) :
+/-- Renaming a variable to itself has no effect. -/
+@[simp]
+lemma Term.rename_same [DecidableEq Var] {m : Term Var} {x : Var} :
+  m.rename x x = m := by
+  induction m <;> grind [vars, rename]
+
+/-- Renaming a used variable changes the set of variables. -/
+@[simp]
+lemma Term.rename_vars_used [DecidableEq Var] {m : Term Var} {x y : Var} :
   x ∈ m.vars → (m.rename x y).vars = m.vars.erase x ∪ {y} := by
   induction m with
-  | var z => grind [Term.vars, Term.rename]
+  | var z => grind [vars, rename]
   | abs z m ih =>
     intro hx
-    by_cases hxm : x ∈ m.vars <;> grind [Term.vars, Term.rename, Term.rename_unused]
+    by_cases hxm : x ∈ m.vars <;> grind [vars, rename, rename_unused]
   | app m n ihm ihn =>
     intro hx
     by_cases hxm : x ∈ m.vars
     · by_cases hxn : x ∈ n.vars
-      · grind [Term.vars, Term.rename]
-      · grind [Term.vars, Term.rename, Term.rename_unused]
+      · grind [vars, rename]
+      · grind [vars, rename, rename_unused]
     · have hxn : x ∈ n.vars := by
-        grind [Term.vars]
-      grind [Term.vars, Term.rename, Term.rename_unused]
+        grind [vars]
+      grind [vars, rename, rename_unused]
+
+/-- Renaming removes the variable. -/
+lemma Term.rename_remove [DecidableEq Var] {m : Term Var} {x y : Var} :
+  x ≠ y → x ∉ (m.rename x y).vars := by
+  intro hxy
+  by_cases hx : x ∈ m.vars <;> grind [rename_vars_used, rename_unused]
+
+/-- Renaming changes set of variables. -/
+lemma Term.rename_vars [DecidableEq Var] {m : Term Var} {x y : Var} :
+  (m.rename x y).vars ⊆ m.vars \ {x} ∪ {y} := by
+  by_cases x ∈ m.vars <;> grind [vars, rename, rename_unused, rename_vars_used]
 
 /-- Concatenation of renaming. -/
-lemma Term.rename_concat [DecidableEq Var] (m : Term Var) (x y z : Var) :
+@[simp]
+lemma Term.rename_concat [DecidableEq Var] {m : Term Var} {x y z : Var} :
   y ∉ m.vars → (m.rename x y).rename y z = m.rename x z := by
-  induction m <;> grind [Term.vars, Term.rename]
+  induction m <;> grind [vars, rename]
+
+/-- Commutativity of renaming. -/
+@[simp]
+lemma Term.rename_comm [DecidableEq Var] {m : Term Var} {x y z w : Var} :
+  x ≠ z → y ∉ m.vars ∪ {x, z} → w ∉ m.vars ∪ {x, z} →
+  (m.rename x y).rename z w = (m.rename z w).rename x y := by
+  induction m <;> grind [vars, rename]
+
+/-- α-equivalent terms have the same size. -/
+lemma AlphaEquiv.eq_sizeOf [DecidableEq Var] {m n : Term Var} :
+  m =α n → sizeOf m = sizeOf n := by
+  intro h
+  induction h with
+  | @var x => rfl
+  | @abs y x1 x2 m1 m2 hy h ih =>
+    simpa using ih
+  | @app m1 n1 m2 n2 _ hm hn =>
+    grind [app.sizeOf_spec]
+
+/-- Reflexivity of α-equivalence. -/
+lemma AlphaEquiv.refl [DecidableEq Var] [HasFresh Var] (m : Term Var) : m =α m := by
+  refine WellFounded.induction (C := fun m => m =α m) sizeOfWFRel.wf m ?_
+  simp only; intro m ih
+  cases m with
+  | var x => apply AlphaEquiv.var
+  | abs x m =>
+    obtain ⟨z, hz⟩ := HasFresh.fresh_exists (m.vars ∪ {x})
+    apply AlphaEquiv.abs (y := z) (x1 := x) (x2 := x) (m1 := m) (m2 := m)
+    <;> try grind [rename_unused, rename_vars, rename_concat]
+    · apply ih
+      change sizeOf (m.rename x z) < sizeOf (abs x m)
+      grind [rename.eq_sizeOf, abs.sizeOf_spec]
+  | app m n =>
+    apply AlphaEquiv.app
+    · apply ih
+      change sizeOf m < sizeOf (app m n)
+      grind [rename.eq_sizeOf, app.sizeOf_spec]
+    · apply ih
+      change sizeOf n < sizeOf (app m n)
+      grind [rename.eq_sizeOf, app.sizeOf_spec]
+
+/-- Symmetry of α-equivalence. -/
+lemma AlphaEquiv.symm [DecidableEq Var] [HasFresh Var] {m n : Term Var} :
+  m =α n → n =α m := by
+  intro h
+  induction h with
+  | @var x => apply AlphaEquiv.var
+  | @abs y x1 x2 m1 m2 hy h ih =>
+    apply AlphaEquiv.abs (y := y) (x1 := x2) (x2 := x1) (m1 := m2) (m2 := m1)
+    <;> try grind [rename_unused, rename_vars, rename_concat]
+    · apply ih
+  | @app m1 n1 m2 n2 hwm1 hwn1 hwm2 hwn2 =>
+    apply AlphaEquiv.app <;> assumption
+
+/-- Renaming under an abstraction body can be reordered against the outer renaming.
+    This lemma is used for the lemma below. -/
+lemma Term.rename_abs_body_comm [DecidableEq Var] {m : Term Var} {x y z w : Var} :
+  y ∉ m.vars ∪ {x, z} → w ∉ m.vars ∪ {x, y, z} →
+  (m.rename x y).rename (if z = x then y else z) w = (m.rename z w).rename x y := by
+  intro hy hw
+  by_cases hzx : z = x
+  · grind [rename_same, rename_unused, rename_concat, rename_vars]
+  · grind [rename_comm]
+
+/-- Renaming α-equivalent terms produces α-equivalent terms. -/
+lemma AlphaEquiv.rename_preserve [DecidableEq Var] [HasFresh Var]
+  (m n : Term Var) (x y : Var) :
+  y ∉ m.vars ∪ n.vars → m =α n → (m.rename x y) =α (n.rename x y) := by
+  refine (WellFounded.induction sizeOfWFRel.wf m
+    (C := fun m => ∀ (n : Term Var) (x y : Var), y ∉ m.vars ∪ n.vars →
+      m =α n → (m.rename x y) =α (n.rename x y)) ?_) n x y
+  intro m ih n x y hy h
+  by_cases hxy : y = x
+  · grind [rename_same]
+  cases h with
+  | @var z => apply AlphaEquiv.refl
+  | @abs z x1 x2 m1 m2 hz hbody =>
+    obtain ⟨w, hw⟩ := HasFresh.fresh_exists (m1.vars ∪ m2.vars ∪ {x1, x2, x, y, z})
+    apply AlphaEquiv.abs (y := w) <;> try grind [rename_vars]
+    rw [rename_abs_body_comm, rename_abs_body_comm] <;> try grind [vars]
+    apply ih <;> try grind [vars, rename_vars]
+    · change sizeOf (m1.rename x1 w) < sizeOf (abs x1 m1)
+      grind [rename.eq_sizeOf, abs.sizeOf_spec]
+    · have hxzw : ((m1.rename x1 z).rename z w) =α ((m2.rename x2 z).rename z w) := by
+        apply ih <;> try grind [vars, rename_vars]
+        · change sizeOf (m1.rename x1 z) < sizeOf (abs x1 m1)
+          grind [rename.eq_sizeOf, abs.sizeOf_spec]
+        · assumption
+      grind [rename_concat]
+  | @app m1 n1 m2 n2 hm hn =>
+    apply AlphaEquiv.app
+    · apply ih m1 <;> try grind [vars]
+      · change sizeOf m1 < sizeOf (app m1 m2)
+        grind [app.sizeOf_spec]
+      · assumption
+    · apply ih m2 <;> try grind [vars]
+      · change sizeOf m2 < sizeOf (app m1 m2)
+        grind [app.sizeOf_spec]
+      · assumption
+
+/-- Elimination rule for α-equivalence of abstractions.
+    It states that if two abstractions are α-equivalent,
+    then their bodies can be renamed to ``any'' fresh variable y and remain α-equivalent.
+    This is sometimes easier to use than using by_cases on the equivalence,
+    which can only produce the claim for ``some'' fresh y. -/
+lemma AlphaEquiv.abs_elim [DecidableEq Var] [HasFresh Var] {m1 m2 : Term Var} {x1 x2 y : Var} :
+  y ∉ m1.vars ∪ m2.vars ∪ {x1, x2} → (abs x1 m1) =α (abs x2 m2) →
+  (m1.rename x1 y) =α (m2.rename x2 y) := by
+  intro hy h
+  cases h with
+  | @abs z _ _ _ _ hz h1 =>
+    by_cases hzy : z = y
+    · subst z
+      assumption
+    · have hxzy : ((m1.rename x1 z).rename z y) =α ((m2.rename x2 z).rename z y) := by
+        apply AlphaEquiv.rename_preserve <;> try grind [AlphaEquiv.rename_preserve, rename_vars]
+        assumption
+      grind [rename_concat, rename_vars]
+
+/-- Transitivity of α-equivalence. -/
+lemma AlphaEquiv.trans [DecidableEq Var] [HasFresh Var] {m n p : Term Var} :
+  m =α n → n =α p → m =α p := by
+  refine (WellFounded.induction sizeOfWFRel.wf m
+    (C := fun m => ∀ (n p : Term Var),
+      m =α n → n =α p → m =α p) ?_) n p
+  intro m ih n p hmn hnp
+  cases m with
+  | var x =>
+    cases hmn with
+    | @var x => assumption
+  | abs x1 m1 =>
+    obtain ⟨w, hw⟩ := HasFresh.fresh_exists (m1.vars ∪ {x1} ∪ n.vars ∪ p.vars)
+    have hmn' := hmn
+    cases hmn' with
+    | @abs y x1 x2 m1 m2 hy h1 =>
+      have hnp' := hnp
+      cases hnp' with
+      | @abs z x2 x3 m2 m3 hz h2 =>
+        apply AlphaEquiv.abs (y := w)
+        <;> try grind [vars, rename_unused, rename_vars, rename_concat]
+        · apply ih _ ?_ (m2.rename x2 w) <;> try grind [AlphaEquiv.abs_elim, vars, rename_vars]
+          change sizeOf (m1.rename x1 w) < sizeOf (abs x1 m1)
+          grind [rename.eq_sizeOf, abs.sizeOf_spec]
+  | app m1 m2 =>
+    cases hmn with
+    | @app m1 n1 m2 n2 hmn1 hmn2 =>
+      cases hnp with
+      | @app n1 p1 n2 p2 hnp1 hnp2 =>
+        apply AlphaEquiv.app
+        · apply ih _ ?_ n1 <;> try assumption; try grind [vars, rename_vars]
+          change sizeOf m1 < sizeOf (app m1 m2)
+          grind [app.sizeOf_spec]
+        · apply ih _ ?_ n2 <;> try assumption; try grind [vars, rename_vars]
+          change sizeOf m2 < sizeOf (app m1 m2)
+          grind [app.sizeOf_spec]
+
+/-- Renaming a non-free variable result in an α-equivalent term. -/
+lemma AlphaEquiv.rename_non_fv [DecidableEq Var] [HasFresh Var] (m : Term Var) (x y : Var)
+  (hxm : x ∉ m.fv) (hym : y ∉ m.vars) : m =α (m.rename x y) := by
+  induction m with
+  | var z =>
+    have hzx : z ≠ x := by
+      grind [fv]
+    simpa [rename, hzx] using AlphaEquiv.var
+  | abs z m ih =>
+    by_cases hzx : z = x
+    · subst z
+      simp only [rename, ↓reduceIte]
+      obtain ⟨w, hw⟩ := HasFresh.fresh_exists (m.vars ∪ {x, y})
+      apply AlphaEquiv.abs (y := w)<;> try grind [rename_unused, rename_vars]
+      rw [rename_concat] <;> try grind [vars]
+      apply AlphaEquiv.refl
+    · simp only [rename, hzx, ↓reduceIte]
+      obtain ⟨w, hw⟩ := HasFresh.fresh_exists (m.vars ∪ {x, y, z})
+      apply AlphaEquiv.abs (y := w) <;> try grind [rename_unused, rename_vars]
+      apply AlphaEquiv.rename_preserve <;> grind [vars, rename_vars, fv]
+  | app m1 m2 ih1 ih2 =>
+    apply AlphaEquiv.app
+    · apply ih1 <;> grind [vars, fv]
+    · apply ih2 <;> grind [vars, fv]
+
+/-- Any `Term` can be obtained by filling a `Context` with a variable. This proves that `Context`
+completely captures the syntax of terms. -/
+theorem Context.complete (m : Term Var) :
+    ∃ (c : Context Var) (x : Var), m = (c.fill (Term.var x)) := by
+  induction m with
+  | var x => exists hole, x
+  | abs x n ih =>
+    obtain ⟨c', y, ih⟩ := ih
+    exists Context.abs x c', y
+    rw [ih, fill]
+  | app n₁ n₂ ih₁ ih₂ =>
+    obtain ⟨c₁, x₁, ih₁⟩ := ih₁
+    exists Context.appL c₁ n₂, x₁
+    rw [ih₁, fill]
+
 
 end LambdaCalculus.Named
 
